Started adding lemmas to the Monad version

Monad_Play Around/DNFP/Dutch_National_Flag_Monad.thy
@@ -6,6 +6,7 @@ imports
 begin
 
 text\<open>Monad definitions to encode and extract data from the monad\<close>
+datatype color = red | white | blue
 
 record env = 
   high :: "nat"
@@ -16,6 +17,8 @@ record env =
 definition return:: "'a \<Rightarrow> ('b, 'a) state" where "return = State_Monad.return"
 definition get:: "(env, env) state" where "get = State (\<lambda>x. (x,x))"
 definition put:: "env \<Rightarrow> (env, unit) state" where "put x = State (\<lambda>_. ((),x))"
+text\<open>Ask Stefan about how to do generic get\<close>
+definition get_gen:: "char list\<Rightarrow> (env, 'a) state" where "get_gen acc = do { x \<leftarrow> get; return (acc  x)}"
 
 definition get_high:: "(env, nat) state" where "get_high = do { x \<leftarrow> get; return (high  x) }" 
 definition get_low:: "(env, nat) state" where "get_low = do { x \<leftarrow> get; return (low x) }" 
@@ -27,7 +30,6 @@ definition set_high:: "env \<Rightarrow> nat \<Rightarrow> env" where "set_high 
              low = low v,
              i = i v,
              xs = xs v \<rparr>"
-
 definition set_low:: "env \<Rightarrow> nat \<Rightarrow> env" where "set_low v x =  
 \<lparr>            high = high v,
              low = x,
@@ -65,59 +67,55 @@ lemma distinct_swap[simp]:
 
 value\<open>swap [a,b,c,d,e] 0 4 = [e,b,c,d,a]\<close>
 
-text\<open>The algorithm is constant so n is originally defined as the size of the list.
-      s is the list I am sorting
-      low is the bound of sorted array
-      i is the current element being investigated\<close>
-fun dnfp:: "nat \<Rightarrow> nat list \<Rightarrow> nat \<Rightarrow> nat \<Rightarrow> nat \<Rightarrow> nat list" where
-"dnfp 0 s _ _ _ = s"|
-"dnfp (Suc 0) s _ _ _ = s"|
-"dnfp (Suc n) s l h j = (if h > j then (if s!j < 1 then (dnfp n (swap s j l) (Suc l) h (Suc j))
-                                else (if s!j > 1 then (dnfp n (swap s j (h-1)) l (h-1) j)
-                                  else (dnfp n s l h (Suc j))))
-                             else s)"
+definition init_loop where
+"init_loop \<equiv> do{
+                  h \<leftarrow> get_high;
+                  i \<leftarrow> get_i;
+                  s \<leftarrow> get_xs;
+                  return (h, i, s)
+                }"
 
-text\<open>Is this better - with the let and (Suc high)?\<close>
-fun dnfp1:: "nat \<Rightarrow> nat list \<Rightarrow> nat \<Rightarrow> nat \<Rightarrow> nat \<Rightarrow> nat list" where
-"dnfp1 0 s _ _ _ = s"|
-"dnfp1 (Suc 0) s _ _ _ = s"|
-"dnfp1 (Suc n) s l (Suc h) j = (if (Suc h) > j then (
-                                  let (xs, l1, h1, j1) = (if s!j < 1 then ((swap s j l), (Suc l), (Suc h), (Suc j))
-                                                 else (if s!j > 1 then ((swap s j h), l, h, j)
-                                                 else (s, l, (Suc h), (Suc j))))
-                                  in (dnfp1 n xs l1 h1 j1))
-                             else s)"
+definition inc_lowbound where
+"inc_lowbound s x\<equiv> do{
+                  l \<leftarrow> get_low;                                       
+                  put_xs (swap s x l);
+                  put_i (Suc x);
+                  put_low (Suc l)
+                }"
+
+definition dec_highbound where
+"dec_highbound s j h\<equiv> do{
+                    put_high (h - 1);
+                    put_xs (swap s j (h-1))
+                }"
+
+definition loop_update_action where
+"loop_update_action s j h \<equiv> 
+do{
+  (if s!j < 1 then do {
+    inc_lowbound s j
+  }else (if s!j > 1 then do
+  {
+    dec_highbound s j h
+  }
+   else do {
+     put_i (Suc j)
+   }))
+}"
 
 text\<open>A version using a state monad for storing the list/array that is being sorted\<close>
+(*\<comment> l < high \<and> i < h*)
 fun dnfp_mon:: "nat \<Rightarrow> (env, unit) state" where
 "dnfp_mon 0  = skip"|
 "dnfp_mon (Suc 0)  = skip"|
-"dnfp_mon (Suc n)  = do{
-                        h \<leftarrow> get_high;
-                        i \<leftarrow> get_i;
-                        s \<leftarrow> get_xs;
-                        (if h > i then
-                                do{
-                                  (if s!i < 1 then do {
-                                            l \<leftarrow> get_low;                                       
-                                            put_xs (swap s i l);
-                                            put_i (Suc i);
-                                            put_low (Suc l);
-                                            dnfp_mon n
-                                          }
-                                   else (if s!i > 1 then do
-                                          {
-                                            put_high (h - 1);
-                                            put_xs (swap s i (h-1));
-                                            dnfp_mon n
-                                          }
-                                       else do {
-                                         put_i (Suc i);
-                                        dnfp_mon n
-                                       }))
-                                }
-                             else skip)
-                      }"
+"dnfp_mon (Suc n)  = do {
+                      (h, i, s) \<leftarrow> init_loop;
+                        (if h > i then do{
+                          loop_update_action s i h;
+                          dnfp_mon n
+                         }
+                       else skip
+                      )}"
 
 definition init_env:: "nat list \<Rightarrow> env" where
   "init_env l \<equiv> \<lparr>high = (length l),            low = 0,
@@ -128,12 +126,62 @@ definition init_state_env:: "nat list \<Rightarrow> (env, unit) state" where
 
 value \<open>snd(run_state (dnfp_mon 5) (init_env [0,2,2,1,2]))\<close>
 value \<open>snd(run_state (dnfp_mon 9) (init_env [0,2,2,0,1,0,2,1,2]))\<close>
-value \<open>snd(run_state (dnfp_mon 3)(init_env[2,1,0]))\<close>
+value \<open>snd(run_state (dnfp_mon 3)(init_env [2,1,0]))\<close>
 
 value \<open>sorted(xs(snd(run_state (dnfp_mon 5) (init_env[0,2,2,1,2]))))\<close>
 value \<open>sorted(xs(snd(run_state (dnfp_mon 9) (init_env[0,2,2,0,1,0,2,1,2]))))\<close>
 value \<open>sorted(xs(snd(run_state (dnfp_mon 3) (init_env[2,1,0]))))\<close>
 
+
+section\<open>Pre and postconditions\<close>
+
+lemma inc_lowbound_post:
+"\<lbrakk>init_env l = e; length l = Suc n; low e = l1; i e = j1; high e = h1; 
+    h1 > j1; l!j1 < 1 ; snd (run_state (inc_lowbound l j1) e) = e2; high e2 = h2; i e2 = j2\<rbrakk> \<Longrightarrow> (h2 - j2) \<le> (h1 - j1)"
+  apply(simp_all add: snd_def inc_lowbound_def get_low_def return_def swap_def put_i_def put_def)
+  apply(simp_all add: put_low_def set_i_def set_low_def get_def put_def put_xs_def set_xs_def)
+  apply(simp_all add: low_def Record.iso_tuple_snd_def Record.iso_tuple_fst_def fst_def env_ext_Tuple_Iso_def Record.tuple_iso_tuple_def snd_def)
+  apply(simp add: init_env_def low_def high_def Record.iso_tuple_fst_def fst_def Record.tuple_iso_tuple_def env_ext_Tuple_Iso_def)
+   apply(simp_all only: repr_def iso_tuple_snd_def low_def high_def Record.iso_tuple_fst_def fst_def Record.tuple_iso_tuple_def env_ext_Tuple_Iso_def)
+  apply(simp_all add: id_def)
+  sledgehammer
+  sorry
+
+
+text\<open>The difference between high and i will never increase and will be decreased by loop_update_action\<close>
+lemma termination_loop_update_action:
+"\<lbrakk>init_env l = e; length l = Suc n; high e = h1; i e = j1; h1 > j1 ; snd (run_state (loop_update_action l j1 h1) e) = e2; high e2 = h2; i e2 = j2\<rbrakk> \<Longrightarrow> (h2 - j2) \<le> (h1 - j1)"
+  apply(simp_all add: snd_def high_def init_env_def i_def Record.iso_tuple_fst_def Record.tuple_iso_tuple_def fst_def Record.iso_tuple_snd_def)
+   apply(simp_all add: Record.repr_def env_ext_Tuple_Iso_def)
+  apply(simp_all add: loop_update_action_def inc_lowbound_def inc_lowbound_post dec_highbound_def put_i_def)
+   apply(simp only: loop_update_action_def inc_lowbound_def dec_highbound_def put_i_def)
+   apply(simp only: put_xs_def get_def get_low_def get_high_def put_def return_def put_low_def set_i_def set_xs_def put_high_def)
+  apply(simp only: set_low_def swap_def return_def set_high_def high_def low_def )
+  sorry
+
+
+lemma termination_loop_update_action:
+"\<lbrakk>init_env l = e; high e = h1; i e = j1; h1 > j1 ; h1 - j1 = dif1; snd (run_state (loop_update_action l j1 h1) e) = e2; high e2 = h2; i e2 = j2\<rbrakk> \<Longrightarrow> (h2 - j2) < (h1 - j1) "
+
+
+
+text\<open>Would you add your condition to the assumptions?
+     I mean would you extract low and make sure all elements before low are 0?\<close>
+lemma low_and_down_is_0:
+"\<lbrakk>init_env l = e;  low e = l1; \<forall>x:: nat. x < l1 \<Longrightarrow> l!x = 0; l!j = 0; low(snd (run_state (inc_lowbound l j) e)) = l2\<rbrakk> \<Longrightarrow> l1 < l2 "
+  sorry
+
+lemma low_to_i_is_1:
+"\<lbrakk>dfs1_dfs_dom (Inl (x, e)); black e = bl1; black (snd (run_state (dfs1 x) e)) = bl2 \<rbrakk> \<Longrightarrow> bl1 \<subseteq> bl2"
+  sorry
+
+lemma i_to_high_is_nonsorted:
+"\<lbrakk>dfs1_dfs_dom (Inl (x, e)); black e = bl1; black (snd (run_state (dfs1 x) e)) = bl2 \<rbrakk> \<Longrightarrow> bl1 \<subseteq> bl2"
+  sorry
+
+lemma high_and_up_is_2:
+"\<lbrakk>dfs1_dfs_dom (Inl (x, e)); black e = bl1; black (snd (run_state (dfs1 x) e)) = bl2 \<rbrakk> \<Longrightarrow> bl1 \<subseteq> bl2"
+  sorry
 
 lemma length_dnfp: "length(dnfp n xs k j k) = length xs"
   apply(induction n)
